---
title: "Sequences of real numbers"

categories:
  - Analysis


tags:
  - triangular inequality
  - convergent sequence
  - limit theorems
  - squeeze theorem

toc: true
toc_sticky: true 

use_math : true
comments : true

---
## Theorem 2.1.3 (Triangular inequality)
For all $x,y\in \mathbb{R}, \lvert x+y\rvert\leq \vert x\rvert+\vert y\rvert$

<*Proof*>

$$
\begin{align*}
0\leq (x+y)^2 &=x^2+2xy + y^2 \\
&\leq \lvert x\rvert^2 + 2\lvert x\rvert\cdot \lvert y\rvert + \lvert y\rvert^2 =(\lvert x\rvert+\lvert y\rvert)^2
\end{align*}
$$

Thus, 

$$
\begin{align*}
\lvert x+y\rvert = \sqrt{(x+y)^2} \leq \sqrt{(\lvert x\rvert+\vert y\rvert)^2} = \lvert x\rvert +\lvert y\rvert
\end{align*}
$$

$$\tag*{$\square$}$$

## Corollary 2.1.4
For all $x,y,z\in \mathbb{R}$, we have 

$$
\begin{align}
\lvert x-y\rvert&\leq \lvert x-z\rvert +\lvert z-y\rvert \\
\lvert \lvert x\rvert-\lvert y\rvert \rvert &\leq \lvert x-y\rvert
\end{align}
$$ 


<*Proof*>

(1) By triangular inequality,  

$$
\begin{align*}
\lvert x-y\rvert = \lvert (x-z) + (z-y) \rvert \leq \lvert x-z\rvert+\lvert z-y\rvert
\end{align*}
$$

(2) By triangular inequality, $\lvert x\rvert = \lvert x-y+y\rvert \leq \lvert x-y\rvert+\lvert y\rvert$
Thus, $\lvert x\rvert-\lvert y\rvert \leq \lvert x-y\rvert$. Similarly,

$$
\begin{align*}
\lvert y \rvert= \lvert y-x+x\rvert \leq \lvert x-y\rvert + \lvert x\rvert
\end{align*}
$$

So, $\lvert y\rvert-\lvert x\rvert \leq \lvert x-y\rvert$.

$\therefore \lvert\lvert x\rvert-\lvert y\rvert\rvert\leq \lvert x-y\rvert$ 

$$\tag*{$\square$}$$

## Definition 2.1.5
$d: \mathbb{R}\times\mathbb{R}\to\mathbb{R}$ is **metric** 

(1) $d(x,y) \geq 0, d(x,y) = 0 \iff x=y$ 

(2) $d(x,y) = d(y,x)$ 

 (3) $d(x,y) \leq d(x,z) + d(y,z)$

## Definition 2.1.6 
Let $p \in \mathbb{R}$ and let $\epsilon >0$. The set 

$$
\begin{align*}
N_\epsilon (p) &:=\{ x\in \mathbb{R}: \lvert x-p\rvert<\epsilon \} \\
&= \{x\in\mathbb{R}: p-\epsilon <x<p+\epsilon\} \\
&=(p-\epsilon,p+\epsilon)
\end{align*}
$$

is called an $\epsilon$-neighborhood of the point $p$.

## Definition 2.1.7
A sequence $(p_n)_{n=1}^\infty$ in $\mathbb{R}$ is said to **converge** ,

If $\exists p\in\mathbb{R}$ such that $\forall \epsilon >0, \exists N\in\mathbb{N}$ such that $n\geq N \Rightarrow \lvert p_n-p\rvert<\epsilon\: (\iff p_n \in N_\epsilon (p))$.  We write 

$$
\begin{align}
\lim_{n\to\infty} p_n = p
\end{align}
$$

$(p_n )_{n=1}^\infty$ diverges if it does not converge.

## Theorem
Let $(p_n)_{n=1}^\infty$ be a sequence in metric space $(X,d)$.  $p_n$ converges to $p\in X$ if and only if  for every $r>0, N_r(p)$ contains almost all of the $(p_n)_{n=1}^\infty$, i.e., the neighborhood contains all but a finite number of $(p_n)_{n=1}^\infty$.

<*proof*>

$\Rightarrow$ Suppose that $p_n\to p$ as $n\to\infty$. Let $\epsilon>0$ be given. There exists $N\in\mathbb{N}$ such that $n\geq N \Rightarrow p_n\in N_\epsilon (p).$ Thus, there are $N-1$ points that lie outside of $N_\epsilon (p)$.

$\Leftarrow$ Suppose that any $N_\epsilon (p)$ contains almost all of the $(p_n)_{n=1}^\infty$ and only a finite number of $(p_n)_{n=1}^\infty$ lie outside of $N_\epsilon (p)$. Let $\epsilon >0$ be given. Let $N$ be the greatest index of those who lie outside of $N_\epsilon (p)$. Then if $n\geq N+1$, then $p_n\in N_\epsilon (p)$. 

$\therefore p_n\to p$

$$\tag*{$\square$}$$

## Examples 2.1.8
(a) $\displaystyle{\lim_{n\to\infty}\frac{1}{n} = 0}$

<*proof*>

Let $\epsilon >0$ be given. By Archimedean property, we can find $N\in\mathbb{N}$ s.t. $\frac{1}{N}< \epsilon$. If $n\geq N$, then $\lvert \frac{1}{n}\rvert=\frac{1}{n} \leq \frac{1}{N} <\epsilon$.

$\therefore \displaystyle{\lim_{n\to\infty}\frac{1}{n} = 0}$
$$\tag*{$\square$}$$

(b) $\displaystyle{\lim_{n\to\infty}\frac{2n+1}{3n+2}=\frac{2}{3}}$

<*proof*>

Let $\epsilon >0$ be given. By Archimedean property, $\exists N\in\mathbb{N}$ s.t. $\frac{1}{9N}<\epsilon$. If $n\geq N$, then 

$$
\begin{align*}
\left\lvert\frac{2n+1}{3n+2} -\frac{2}{3}\right\rvert = \frac{1}{3(3n+2)} < \frac{1}{9n} \leq \frac{1}{9N} < \epsilon
\end{align*}
$$

$\therefore \displaystyle{\frac{2n+1}{3n+2}=\frac{2}{3}}$
$$\tag*{$\square$}$$

## Definition 2.1.9
A sequence $(p_n)_{n=1}^\infty$ in $\mathbb{R}$ is said to be **bounded** if there exists a constant $M>0$ such that $\lvert p_n\rvert\leq M$ for all $n\in\mathbb{N}$.

## Lemma 1
Let $a\in \mathbb{R}$ be a real number. If $\lvert a\rvert < \epsilon, \forall \epsilon >0$, then $a=0$.

<*proof*>

Assume that $a\neq 0$, i.e. $\lvert a\rvert >0$. Take $\epsilon_0 := \lvert a\rvert$. Then $\lvert a\rvert < \epsilon_0 = \lvert a\rvert$, which is a contradiction.

$\therefore a= 0$
$$\tag*{$\square$}$$

## Theorem 2.1.10
(a) If a sequence $(p_n)_{n=1}^\infty$ converges, then its limit is unique 

(b) Every convergent sequence in $\mathbb{R}$ is bounded.

<*proof*>

(a) Suppose that $p_n\to L_1, p_n \to L_2$ as $n\to\infty$. Let $\epsilon >0$ be given. 

 Then there exists $N_1, N_2\in\mathbb{N}$ such that 

$$
\begin{align*}
n\geq N_1 &\Rightarrow \lvert p_n-L_1\rvert <\epsilon/2 \\
n\geq N_2 &\Rightarrow \lvert p_n-L_2\rvert <\epsilon/2 \\
\end{align*}
$$

Take 
$$
\begin{align*}
N:=\max\{N_1, N_2\} 
\end{align*}
$$

If $n\geq N$, then 

$$
\begin{align*}
\lvert L_1-L_2\rvert \leq \vert p_n-L_1\rvert + \vert p_n-L_2\rvert < \frac{\epsilon}{2} +\frac{\epsilon}{2} = \epsilon
\end{align*}
$$

Since $\epsilon >0$ was arbitrary, $L_1 = L_2$ by lemma 1.

$$\tag*{$\square$}$$

(b) Let $p_n \to L$. Then there is a $N\in\mathbb{N}$ s.t. $n> N \Rightarrow \lvert p_n -L\rvert <1$. Now, 

$$
\begin{align*}
\lvert p_n\rvert -\lvert L\rvert \leq \lvert p_n-L\rvert < 1
\end{align*}
$$

So, $\lvert p_n\rvert <\lvert L\rvert+1$. Define 
$$
\begin{align*}
M:= \max\{ \lvert p_1\rvert, \ldots, \lvert p_N\rvert, \lvert L\rvert+1\} > 0.
\end{align*}
$$ 

Then $\lvert p_n\rvert \leq M$ for all $n\in M$.

$\therefore (p_n)_{n=1}^\infty$ is bounded

$$\tag*{$\square$}$$

## Theorem 2.2.1 
$\displaystyle{\lim_{n\to\infty}a_n=a, \lim_{n\to\infty}b_n=b}$

(a) $\displaystyle{\lim_{n\to\infty}(a_n+b_n)= a + b}$ 

(b) $\displaystyle{\lim_{n\to\infty}a_n\cdot b_n = ab}$ 

 (c) $a\neq 0, a_n \neq 0, \forall n\in\mathbb{N} \Rightarrow \displaystyle{\lim_{n\to\infty}\frac{b_n}{a_n}= \frac{b}{a}}$

<*proof*>

(a) Let $\epsilon >0$ be given. There exists $N\in\mathbb{N}$ s.t. $n\geq N \Rightarrow \lvert a_n-a\rvert < \frac{\epsilon}{2}, \lvert b_n-b\rvert<\frac{\epsilon}{2}$. If $n\geq N$, then

$$
\begin{align*}
\lvert (a_n+b_n) -(a+b)\rvert &= \lvert a_n-a+b_n-b\rvert \\
&\leq \lvert a_n-a\rvert + \lvert b_n-b\rvert \\
&<\frac{\epsilon}{2} + \frac{\epsilon}{2} = \epsilon
\end{align*}
$$

$\therefore \displaystyle{\lim_{n\to\infty}(a_n+b_n) = a+b}$ 

$$\tag*{$\square$}$$

(b) Let $\epsilon >0$ be given. Since $(a_n)_{n=1}^\infty$ converges, $(a_n)_{n=1}^\infty$ is a bounded sequence so that we can find $M>0$ s.t. $\lvert a_n\rvert \leq M$ for all $n\in \mathbb{N}$.  

By our assumption, there exists $N\in\mathbb{N}$ s.t. $n\geq N\Rightarrow \lvert a_n-a\rvert<\frac{\epsilon}{\lvert b\rvert}$ and $\lvert b_n-b\rvert < \frac{\epsilon}{2M}$. If $n\geq N$, then

$$
\begin{align*}
\lvert a_nb_n -ab\rvert &= \lvert a_n b_n- a_nb + a_nb -ab\rvert  \\
&\leq \lvert a_n\rvert\lvert b_n-b\rvert + \lvert b\rvert\lvert a_n -a\rvert \\
&\leq M\lvert b_n-b\rvert + \lvert b\rvert \lvert a_n-a\rvert \\
&< M \cdot \frac{\epsilon}{2M} + \lvert b\rvert \cdot \frac{\epsilon}{2\lvert b\rvert}\\
&=\frac{\epsilon}{2} + \frac{\epsilon}{2} = \epsilon 
\end{align*}
$$

$\therefore \displaystyle{\lim_{n\to\infty}a_n b_n = b}$
$$\tag*{$\square$}$$

(c) By (b), if suffices to show that $\displaystyle{\lim_{n\to\infty}\frac{1}{a_n}=\frac{1}{a}}$. 

Let $\epsilon >0$ be given. Then, there exists $N_1 \in\mathbb{N}$ such that

$$
\begin{align*}
n\geq N_1 \Rightarrow \lvert a_n-a\rvert <\frac{\lvert a\rvert^2}{2}\epsilon
\end{align*}
$$

Also, there exists $N_2\in \mathbb{N}$such that 

$$
\begin{align*}
n\geq N_2 \Rightarrow \lvert a_n-a\rvert < \frac{\lvert a\rvert}{2}
\end{align*}
$$
Since $\lvert a\rvert-\lvert a_n\rvert \leq \lvert a_n-a\rvert, \lvert a_n\rvert>\frac{\lvert a\rvert}{2}$ for $n\geq N_2$. Put 

$$
\begin{align*}
N:=\max\{ N_1, N_2\} \in \mathbb{N}.
\end{align*}
$$ 

If $n\geq N$,  then 

$$
\begin{align}
\lvert \frac{1}{a_n}=\frac{1}{a}\rvert = \frac{\lvert a_n-a\rvert}{\lvert a_n\rvert\lvert a\lvert} < \frac{2}{\lvert a\rvert^2}\cdot\frac{\lvert a\rvert^2}{2}\epsilon = \epsilon
\end{align}
$$

$\therefore \displaystyle{\lim_{n\to\infty}\frac{1}{a_n}=\frac{1}{a}}$
$$\tag*{$\square$}$$


## Corollary 2.2.
$\displaystyle{\lim_{n\to\infty}a_n = a}, c\in \mathbb{R}$

(a) $\displaystyle{\lim_{n\to\infty}(a_n +c) = a+c }$ 

(b) $\displaystyle{\lim_{n\to\infty}ca_n = ca}$

## Theorem 2.2.3
Let $\displaystyle{\lim_{n\to\infty}a_n=0}$ and let $(b_n)_{n=1}^\infty$ be a bounded sequence. Then $\displaystyle{\lim_{n\to\infty}a_nb_n=0}$

<*proof*>
Let $\epsilon >0$ be given. Then there exists $N\in\mathbb{N}$ s.t. $n\geq N \Rightarrow \lvert a_n\rvert<\frac{\epsilon}{M}$. If $n\geq N$,

$$
\begin{align*}
\lvert a_n b_n\rvert &= \lvert a_n\rvert\lvert b_n\rvert\\
&\leq \lvert a_n\rvert M \\
&<\frac{\epsilon}{M}\cdot M = \epsilon
\end{align*}
$$
$\therefore \displaystyle{\lim_{n\to\infty}a_nb_n}=0$
$$\tag*{$\square$}$$

## Theorem 2.2.4 (Squeeze theorem)
Suppose the sequence $(a_n)_{n=1}^\infty, (b_n)_{n=1}^\infty,\text{and } (c_n)_{n=1}^\infty$ are sequences of real numbers for which there exists $n_0\in \mathbb{N}$ such that 

$$
\begin{align*}
a_n \leq b_n \leq c_n \text{ for all } n\in \mathbb{N}, n\geq n_0
\end{align*}
$$

and that $\displaystyle{\lim_{n\to\infty}a_n = \lim_{n\to\infty}c_n = L}.$ Then the sequence $(b_n)_{n=1}^\infty$ converges and $\displaystyle{\lim_{n\to\infty}b_n=L}$.

<*proof*>

Let $\epsilon >0$ be given. Then there exists $N_1,N_2\in\mathbb{N}$ such that

$$
\begin{align*}
n\geq N_1 \Rightarrow \lvert a_n-L\rvert <\epsilon \\
n\geq N_2 \Rightarrow \lvert b_n-L\rvert <\epsilon
\end{align*}
$$

Put 

$$
\begin{align*}
N:=\max\{N_1, N_2, n_0\} \in \mathbb{N}.
\end{align*}
$$ 

If $n\geq N$, then
$$
\begin{align*}
L-\epsilon < a_n\leq b_n \leq c_n < L+\epsilon
\end{align*}
$$

So, $\lvert b_n -L\rvert<\epsilon$ for $n\geq N$.

$\therefore \displaystyle{\lim_{n\to\infty}b_n=L}$.
$$\tag*{$\square$}$$

## Theorem 2.2.6
(a) $\displaystyle{\lim_{n\to\infty}\frac{1}{n^p} =0}$, for $p> 0$

 (b) $\displaystyle{\lim_{n\to\infty}\sqrt[n]{p}} =1$ for $p>0$ 
 
 (c) $\displaystyle{\lim_{n\to\infty}\sqrt[n]{n}} = 1$ 

(d) $p>1, \alpha \in\mathbb{R}\Rightarrow \displaystyle{\lim_{n\to\infty}\frac{n^\alpha}{p^n}=0}$ 

 (e) $\lvert p\rvert <1 \Rightarrow \displaystyle{\lim_{n\to\infty}}p^n =0$ 

(f) $p\in\mathbb{R} \Rightarrow \displaystyle{\lim_{n\to\infty}\frac{p^n}{n!}} = 0$


<*proof*> 

(a) Let $\epsilon >0$ be given. By Archimedean property, there exists $N\in\mathbb{N}$ s.t. $\frac{1}{N}< \epsilon^{1/p}$. 

For $n\geq N$,

$$
\begin{align*}
\frac{1}{n}\leq  \frac{1}{N} < \epsilon^{1/p}
\end{align*}
$$
Thus, $\left\lvert\frac{1}{n^p}\right\rvert < \frac{1}{N^p} <\epsilon$.

$\therefore \displaystyle{\lim_{n\to\infty}\frac{1}{n^p}}=0$
$$\tag*{$\square$}$$

(b) Assume $p>1$. Let $\epsilon >0$ be given and let $p:=1+\delta$ for some $\delta>0$. We want to show that 

$$
\begin{align*}
1\leq p^{\frac{1}{n}} \leq 1 + \frac{\delta}{n} \text{ for } n\geq 1
\end{align*}
$$

Suppose $p^\frac{1}{n} > 1 +\frac{\delta}{n}$. Then $p=(p^\frac{1}{n})^n > (1+\frac{\delta}{n})^n$. By Bernoulli inequality, 

$$
\begin{align*}
(1+\frac{\delta}{n})^n \geq 1 + n\cdot\frac{\delta}{n} = 1+\delta
\end{align*}
$$
It implies that  $p> 1+\delta$, which contradicts to the assumption.

$\therefore p^\frac{1}{n} \leq 1+\frac{\delta}{n}$

$\therefore \displaystyle{\lim_{n\to\infty}p^\frac{1}{n}}=1$

Now, assume $0<p<1$. Let $a:=\frac{1}{p}$. Then $a>1$. 

$\therefore \displaystyle{\lim_{n\to\infty}a^\frac{1}{n}}=1$


By the limit theorem,

$$
\begin{align*}
\lim_{n\to\infty}p^\frac{1}{n} = \lim_{n\to\infty} \frac{1}{a^{1/n}} = \frac{1}{1}
\end{align*}
$$

$\therefore \displaystyle{\lim_{n\to\infty}p^{\frac{1}{n}}}=1$

$$\tag*{$\square$}$$

(c) Let $x_n:=\sqrt[n]{n}-1$ for $n\geq 2$. Then

$$
\begin{align}
n=(x_n+1)^n \geq \frac{n(n-1)}{2}x^2_n
\end{align}
$$
Thus, $0<x^2_n \leq \frac{2}{n-1}$, i.e. $0<x_n \leq \sqrt{\frac{2}{n-1}}$.

$\therefore \displaystyle{\lim_{n\to\infty}x_n=0}$

$\therefore \displaystyle{\lim_{n\to\infty}\sqrt[n]{n}=1}$
$$\tag*{$\square$}$$

(d) Let $p:=1+q$ for some $q>0$ and let $k\in\mathbb{N}$ with $k>\alpha$. For $k< n/2$,

$$
\begin{align}
\begin{split}
p^n = (1+q)^n &> {n \choose k}q^k  \\
&=\frac{n(n-1)\cdots(n-k+1)}{k!}q^k \\
&> \frac{n^k}{2^kk!} q^k \:(\because n-k+1 > \frac{n}{2}+1 > \frac{n}{2})\\ 
\end{split}
\end{align}
$$

Thus, 

$$
\begin{align}
0< \frac{n^\alpha}{p^n} <\frac{2^k k!}{q^kn^{k-\alpha}}
\end{align}
$$

 Since $k-\alpha>0, \displaystyle{\lim_{n\to\infty}1/n^{k-\alpha}}=0.$

$\therefore \displaystyle{\lim_{n\to\infty}\frac{n^\alpha}{p^n}} =0$
$$\tag*{$\square$}$$

(e) Let $p=\pm \frac{1}{q}$ for some $q>1$.

$$
\begin{align}
\lvert p^n\rvert = \vert p\rvert^n = \frac{1}{q^n}
\end{align}
$$

$\therefore \displaystyle{\lim_{n\to\infty}}p^n=0$ by (d) where $\alpha=0$.

(f) Let $k\in\mathbb{N}$ with $k>\lvert p\rvert$. For $n>k$

$$
\begin{align*}
\left\lvert\frac{p^n}{n!}\right\rvert &= \frac{\left\lvert p\right\rvert^n}{n!} = \frac{\left\lvert p\right\rvert^n}{(k-1)!k\cdots (n-1)n}\\
&< \frac{\left\lvert p\right\rvert^n}{(k-1)!k^{n-k+1}}\\
&=\frac{k^{k-1}}{(k-1)!}\frac{\left\lvert p\right\rvert^n}{k^n}
\end{align*}
$$ 
Since $0<\frac{\lvert p\rvert}{k}<1, \displaystyle{\lim_{n\to\infty}}\frac{\lvert p\rvert^n}{k}=0$

$\therefore \displaystyle{\lim_{n\to\infty}}\frac{p^n}{n!} = 0$
$$\tag*{$\square$}$$

## Reference
- Manfred Stoll,  **『**Introduction to Real Analysis**』**, Pearson
