---
title: "Group and Ring"

categories:
  - Group
  - Ring

tags:
  - group
  - quotient group
  - normal subgroup
  - ring
  - ideal
  - quotient ring
  - well-defined binary operation
  
  

toc: true
toc_sticky: true

use_math : true
comments : true

---


## Definition 1
$\cdot: G\times G \to G$ is binary operation where we write $x\cdot y =xy$ for $x,y\in G$. 
$(G,\cdot)$ is group if it satisfies the followings
(a) For all $x,y,z \in G$, $(x\cdot y)\cdot z = x\cdot (y\cdot z)$.
(b) $\exists e \in G$, such that $x\cdot e = e\cdot x = x$, for all $x\in G$.
(c) For every $x \in G$, $\exists \hat{x} \in G$ such that $x \hat{x} = \hat{x}x = e$.

## Definition 2
Let $(G,\cdot)$ be a group and $H \subset G$ be a **subgroup** satisfying the three requirements of group as described in Definition 1. We write $(H,\cdot) \leq (G,\cdot)$.

## Definition 3
Let  $(G,\cdot)$ is a group and $(H,\cdot) \leq G$. $H$ is normal subgroup if $g^{-1}hg\in H$ for all $g \in G, h \in H$. We write $H \trianglelefteq G$.




## Definition 4
Let $G$ be a group and $H$ be a subgroup of $G$. For $x \in G$, we define a **coset** as follows:
$$
\begin{align}
xH := \{xh| h\in H\}
\end{align}
$$
We call it left coset ($\because xh \neq hx$ if the group is not abelian).

## Definition 5
Let $(G, \cdot)$ be a group and $(H,\cdot)$ be a  normal subgroup of $G$. Then we define quotient group as follows:
$$
G/H := \{xH| x \in G \}
$$
For notational simplicity,  we write a coset $\overline{x} := xH$.

## Theorem 6
 Let $G$ be a group and $H$ be a subgroup of $G$. For $x,y \in G$,
$$
\begin{align}
xH = yH \iff y^{-1}x \in H
\end{align}
$$

<*proof*>
$\Rightarrow$ Suppose that $xH = yH$. Then $xh_1 = yh_2$ for some $h_1, h_2 \in H$, i.e. $y^{-1}x = h_2 h^{-1}_1 \in H.$

$\Leftarrow$ Suppose that $y^{-1}x \in H$, i.e. $y^{-1}x = h_0$ for some $h_0 \in H$. i.e. $x = yh_0$.

For all $h \in H$, $xh = yh_0h\in yH$.
$\therefore xH \subset yH$.

Similarly, $y=xh^{-1}_0$. For all $h \in H$, $yh=xh^{-1}_0h \in xH$.

$\therefore yH \subset xH.$

$\therefore xH = yH$.

$$\tag*{$\square$}$$

## Theorem 6
Let $G$ be a group and $H$ is a normal subgroup of $G$.  The binary operation $\cdot$ on quotient group $G/H$ is defined as $xH\cdot yH := xyH$. where $x,y \in G$.

Then the binary operation is well defined if and only if  $H$ is a normal subgroup.

<*proof*>
$\Leftarrow$ Suppose that $H$ is a normal subgroup of $G$. 

We want to show that $xH = x^\prime H, yH = y^\prime H \Rightarrow xyH = x^\prime y^\prime H$.
$$
\begin{align}
\begin{split}
(x^\prime y^\prime)^{-1} &= y^{\prime -1}x^{\prime -1} xy \\
&=(y^{\prime -1}y)(y^{\prime -1}x^{\prime -1}xy)
\end{split}
\end{align}
$$
Since $H \trianglelefteq G$, $y^{\prime -1}x^{\prime -1}xy \in H$.

$\therefore (y^{\prime -1}y)(y^{\prime -1}x^{\prime -1}xy) \in H.$

$\therefore$ The binary operation is well defined.

$\Rightarrow$ Take $y = y^\prime = g, x= h, x^\prime = 1.$

Then $y^{\prime -1}x^{\prime -1}xy = g^{-1}hg \in H.$

$\therefore H \trianglelefteq G.$
 
 $$\tag*{$\square$}$$

## Definition 7
$(A, +, \cdot)$ is a ring if 

(a) $(A, +)$ is an abelian group

(b) The binary operation $\cdot$ is associative and distributive over $+$

(c) $\cdot$ is commutative 

(d) $\exists 1 \in A$ such that $x1=1x = x$ for all $x \in A$.

## Note 
1) The identity 1 is unique. 
 $(\because 1^\prime$: another identity in $A \Rightarrow 1= 1^\prime 1 =  1^\prime 1 = 1^\prime$)
 2) $1=0 \iff A = 0$ (zero ring)
  $(\because \Rightarrow ) x\in A, x = x1 = x0 =0. \Leftarrow)$ trivial.$)$
 
 ## Definition 8
 Let $A,B$ be rings. $f: A\to B$ is a **ring homomorphism** if 
 1. $f(x+y) = f(x) + f(y)$
 2. $f(xy) = f(x)f(y)$
 3. $f(1)=1$

## Definition 9
$S \subset (A, +, \cdot)$ is a subring if $(S, +, \cdot)$ is a ring.

## Definition 10
Let $A$ be a ring.  $\mathfrak{a} \subset A$ is an **ideal of $A$**
if $(\mathfrak{a},+) \leq (A, +)$ and $A\mathfrak{a} \subset \mathfrak{a}$, i.e. $[x\in A, y \in \mathfrak{a} \Rightarrow xy \in \mathfrak{a}]$.

## Remark 11
Since $(A, +)$ is abelian and $(\mathfrak{a}, +) \leq (A,+)$, we can think of the quotient group $(A/\mathfrak{a}, +)$. Moreover, we can give a multiplication on $A/\mathfrak{a}$ by 
$$
\overline{x}\cdot\overline{y}:=(x+\mathfrak{a})(y+\mathfrak{a}) := xy + \mathfrak{a}
$$
where $x,y \in A$.

## Theorem 12
Let $A$ be a ring and $J$ be an additive subgroup. 
The binary operation $\overline{x}\cdot\overline{y}:= (x+J)(y+J)$ is well defined if and only if $\mathfrak{a}$ is an ideal, where $x,y \in A$.

<*proof*>
$\Rightarrow$ Suppose that $\overline{x}\cdot\overline{y}$ is well defined where $x,y \in A$. We want to show that for all $a \in A, j\in J$, $aj \in J$. Take $x:=a \in A$ and $y:=0 \in A$. Then, $(a+J)J = J$.
Since $a\in a+J, aj \in (a+J)J = J$. 

$\therefore J$ is an ideal

$\Leftarrow$ Suppose that $J$ is an ideal
We want to show that 
$$
x_1 - x_2 \in J, y_1 -y_2 \in J \Rightarrow x_1y_1 -x_2y_2 \in J
$$
where $x_1, x_2, y_1, y_2 \in J$.
Since $J$ is an ideal and $x_1 - x_2 \in J, y_1 - y_2 \in J$, $y_1(x_1-x_2) \in J, x_2(y_1-y_2) \in J$.
Since $J$ is an additive subgroup,
$$
\begin{align}
\begin{split}
J &\ni y_1(x_1-x_2) + x_2(y_1-y_2) \\
&=y_1x_1 = y_1x_2 + x_2y_1 - x_2y_2 \\
&=x_1y_1 - x_2y_1 + x_2y_1 - x_2y_2 \\
&= x_1y_1 - x_2y_2
\end{split}
\end{align}
$$
The second equality holds because $A$ is  ring so $\cdot$ is commutative.

$\therefore x_1y_1 - x_2y_2 \in J$

 $$\tag*{$\square$}$$


## Reference
- Lecture note from [Hobin Jeong](https://www.youtube.com/watch?v=6PsBsFJgP2Y&list=PL4m4z_pFWq2pMmeQF2tiKzfp7NuAO3sk_&ab_channel=%EC%88%98%ED%95%99%EC%9D%98%EC%A6%90%EA%B1%B0%EC%9B%80%2CEnjoyingMath).
- 이인석, 『선형대수와 군』,서울대학교출판문화원
